cut-elimination in mll

mll.v
@@ -2,9 +2,14 @@ Require Import Lia.
 
 Require Import List_more.
 Require Import List_Type_more.
+Require Import wf_nat_more.
+Require Import PeanoNat.
 
+Require Import List_more2.
+Require Import List_nat.
 Require Import Fun_nat.
 Require Import Perm.
+Require Import Perm_R.
 Require Import misc.
 Require Import Perm_solve.
 
@@ -14,6 +19,14 @@ Inductive formulas : Set :=
 | tens : formulas -> formulas -> formulas
 | parr : formulas -> formulas -> formulas.
 
+Fixpoint fsize A :=
+  match A with
+  | var X => 0
+  | covar X => 0
+  | tens A B => S (fsize A + fsize B)
+  | parr A B => S (fsize A + fsize B)
+  end.
+
 Fixpoint dual A :=
   match A with
   | var X => covar X
@@ -21,6 +34,16 @@ Fixpoint dual A :=
   | tens A B => parr (dual B) (dual A)
   | parr A B => tens (dual B) (dual A)
   end.
+
+Lemma bidual : forall A, dual (dual A) = A.
+Proof with try reflexivity.
+  induction A; simpl; try rewrite IHA1; try rewrite IHA2...
+Qed.
+
+Lemma fsize_dual : forall A, fsize (dual A) = fsize A.
+Proof with try reflexivity.
+  induction A; simpl; try rewrite IHA1; try rewrite IHA2; try rewrite Nat.add_comm...
+Qed.
 
 Inductive mll_cut : list formulas -> Type :=
 | ax_cut_r : forall X, mll_cut (covar X :: var X :: nil)
@@ -39,3 +62,175 @@ Inductive mll : list formulas -> Type :=
 | tens_r : forall A B l1 l2, mll (A :: l1) -> mll (B :: l2) ->
                              mll (tens A B :: l2 ++ l1)
 | parr_r : forall A B l, mll (A :: B :: l) -> mll (parr A B :: l).
+
+Fixpoint psize {l} (pi : mll l) :=
+  match pi with
+  | ax_r _ => 0
+  | ex_r _ _ pi _ _ => S (psize pi)
+  | tens_r _ _ _ _ pi1 pi2 => S (psize pi1 + psize pi2)
+  | parr_r _ _ _ pi => S (psize pi)
+  end.
+
+(* TODO: NEED MOVING *)
+Lemma app_antecedent_dflt {A} : forall (d a : A) f l l1 l2,
+    all_lt f (length l) = true ->
+    app_nat_fun_dflt f l d = l1 ++ a :: l2 ->
+    nth (nth (length l1) f 0) l d = a.
+Proof.
+  intros d a f l l1.
+  revert d a f l.
+  induction l1; intros d b f l l2 Hal Heq.
+  - simpl in *.
+    destruct f; destruct l; try now inversion Heq.
+  - destruct f; [ destruct l; inversion Heq | ].
+    simpl.
+    simpl in Hal; apply andb_prop in Hal as [_ Hal].
+    apply IHl1 with l2; try assumption.
+    destruct l; try now inversion Heq.
+Qed.
+
+Lemma app_antecedent {A} : forall (d a : A) f l l1 l2,
+    all_lt f (length l) = true ->
+    app_nat_fun f l = l1 ++ a :: l2 ->
+    nth (nth (length l1) f 0) l d = a.
+Proof.
+  intros d a f l l1 l2 Hal Heq.
+  apply app_antecedent_dflt with l2; try assumption.
+  destruct l; [ destruct l1; inversion Heq | ].
+  unfold app_nat_fun in Heq.
+  rewrite app_nat_fun_dflt_indep with _ _ _ a0; try assumption.
+Qed.
+
+Lemma cut_admissible : forall A l1 l2,
+    mll (dual A :: l1) ->
+    mll (A :: l2) ->
+    mll (l2 ++ l1).
+Proof with try assumption; try reflexivity.
+  enough (forall c s A l0 l1 l2 (pi1 : mll (dual A :: l0)) (pi2 : mll (l1 ++ A :: l2)),
+          s = psize pi1 + psize pi2 -> fsize A <= c -> mll (l1 ++ l0 ++ l2)) as IH.
+  { intros A l1 l2 pi1 pi2.
+    rewrite <- (app_nil_l _) in pi2.
+    replace (l2 ++ l1) with (app_nat_fun (cfun (length l1) (length l2)) (nil ++ l1 ++ l2)) by (simpl; apply app_cfun_eq).
+    apply ex_r; [ | apply cfun_is_perm | length_lia].
+    refine (IH _ _ A _ _ _ pi1 pi2 _ _)... }
+  induction c as [c IHcut0] using lt_wf_rect.
+  assert (forall A, fsize A < c -> forall l0 l1 l2,
+               mll (dual A :: l0) -> mll (l1 ++ A :: l2) -> mll (l1 ++ l0 ++ l2)) as IHcut by (intros A Hs l0 l1 l2 pi1 pi2 ; refine (IHcut0 _ _ _ _ _ _ _ pi1 pi2 _ _) ; try eassumption; try reflexivity) ;
+    clear IHcut0.
+  induction s as [s IHsize0] using lt_wf_rect.
+  assert (forall A l0 l1 l2 (pi1 : mll (dual A :: l0)) (pi2 : mll (l1 ++ A :: l2)), psize pi1 + psize pi2 < s -> fsize A <= c -> mll (l1 ++ l0 ++ l2))
+    as IHsize by (intros ; eapply IHsize0 ; try eassumption; try reflexivity) ; clear IHsize0.
+  intros A l0 l1 l2 pi1 pi2 Heqs Hc.
+  rewrite_all Heqs ; clear s Heqs.
+  remember (l1 ++ A :: l2) as l ; destruct pi2.
+  - (* ax_r *)
+    destruct l1 ; inversion Heql ; subst.
+    + replace (nil ++ l0 ++ var X :: nil) with (app_nat_fun (cfun 1 (length l0)) (var X :: l0)) by (change (var X :: l0) with ((var X :: nil) ++ l0); change 1 with (length (var X :: nil)); now rewrite app_cfun_eq).
+      apply ex_r ; [ | apply cfun_is_perm | length_lia] ...
+    + unit_vs_elt_inv H1 ; list_simpl...
+  - (* ex_r *)
+    simpl in IHsize.
+    destruct (nth_split_Type (nth (length l1) f 0) l A) as [[la lb] Heq Hlen].
+    + apply andb_prop in e as [Hal _]; rewrite e0 in Hal; apply cond_all_lt_inv...
+      rewrite<- app_nat_fun_length with _ l ; [ | destruct l; [destruct l1; inversion Heql | intros H; inversion H ]].
+      rewrite Heql; length_lia.
+    + rewrite app_antecedent with _ A _ _ _ l2 in Heq ; [ | rewrite<- e0; apply andb_prop in e as [Hal _] | ]...
+      revert pi2 IHsize; rewrite Heq; intros pi2 IHsize.
+      enough (Perm_R (la ++ l0 ++ lb) (l1 ++ l0 ++ l2)) as [p [Hperm [Hlen' Heq']]].
+      { rewrite Heq'; apply ex_r...
+        apply IHsize with A pi1 pi2...
+        lia. }
+      transitivity (l0 ++ l2 ++ l1); [ | rewrite (app_assoc _ _ l1); apply Perm_R_app_comm ].
+      transitivity (l0 ++ lb ++ la); [ rewrite (app_assoc _ _ la); apply Perm_R_app_comm | ]. 
+      apply Perm_R_app_head.
+      transitivity (la ++ lb) ; [ apply Perm_R_app_comm | ].
+      transitivity (l1 ++ l2) ; [ | apply Perm_R_app_comm ].
+      apply Perm_R_app_inv with A.
+      split with f.
+      rewrite<- Heq; repeat split; [ | | symmetry]...
+  - (* tens_r *)
+    destruct l1 ; inversion Heql ; subst ; list_simpl.
+    + (* main case *)
+      remember (dual (tens A0 B) :: l0) as l' ; destruct pi1; try inversion Heql'.
+      * (* ex_r *)
+        remember (tens_r _ _ _ _ pi2_1 pi2_2) as pi2; clear pi2_1 pi2_2 Heqpi2 IHcut.
+        simpl in IHsize.
+        destruct f; [destruct l; inversion H0 | ].
+        destruct (andb_prop _ _ e) as [Hal _]; rewrite e0 in Hal; simpl in Hal; apply andb_prop in Hal as [Hlt Hal]; apply Nat.ltb_lt in Hlt.
+        destruct (nth_split_Type n l A0) as [[la lb] Heq Hlen]...
+        replace (nth n l A0) with (parr (dual B) (dual A0)) in Heq by (destruct l; [ | app_nat_fun_unfold f l n f0; rewrite nth_indep with _ _ _ _ f0; try assumption]; now inversion H0).
+        revert pi1 pi2 IHsize; rewrite Heq; replace (tens A0 B) with (dual (parr (dual B) (dual A0))) by (simpl; now rewrite 2 bidual) ; intros pi1 pi2 IHsize.
+        enough (Perm_R (la ++ (l4 ++ l3) ++ lb) (l0  ++ (l4 ++ l3))) as [p [Hperm [Hlen' Heq']]].
+        { rewrite Heq'; apply ex_r...
+          apply IHsize with  (parr (dual B) (dual A0)) pi2 pi1; [ lia | ].
+          simpl in *; rewrite 2 fsize_dual; lia. }
+        transitivity ((l4 ++ l3) ++ l0); [ | apply Perm_R_app_comm ].
+        transitivity ((l4 ++ l3) ++ lb ++ la); [ rewrite (app_assoc _ _ la); apply Perm_R_app_comm | ]. 
+        apply Perm_R_app_head.
+        transitivity (la ++ lb) ; [ apply Perm_R_app_comm | ].
+        change l0 with (nil ++ l0).
+        apply Perm_R_app_inv with (parr (dual B) (dual A0)).
+        split with (n :: f).
+        rewrite<- Heq; repeat split ; [ | | symmetry]...
+      * (* parr_r *)
+        clear IHsize ; subst.
+        rewrite <- (app_nil_l (A0 :: _)) in pi2_1 ; simpl in Hc ; list_simpl.
+        rewrite <- (bidual B) in pi2_2.
+        refine (IHcut _ _ _ _ _ pi2_2 _)...
+        -- rewrite fsize_dual; lia.
+        -- replace (l0 ++ dual B :: l3) with (app_nat_fun (cfun (length (dual B :: l3)) (length l0)) ((dual B :: l3) ++ l0)) by apply app_cfun_eq.
+           apply ex_r ; [ | apply cfun_is_perm | length_lia ].
+           list_simpl in pi2_1 ; rewrite <- (bidual A0) in pi2_1.
+           change ((dual B :: l3) ++ l0) with ((dual B :: nil) ++ l3 ++ l0).
+           refine (IHcut _ _ _ _ _ pi2_1 _)...
+           rewrite fsize_dual; lia.
+    + (* commutative case *)
+      dichot_Type_elt_app_exec H1 ; subst.
+      * rewrite 2 app_assoc ; apply tens_r...
+        revert pi2_2 IHsize ; simpl ; rewrite (app_comm_cons _ _ B) ; intros pi2_2 IHsize.
+        rewrite <- app_assoc ; refine (IHsize _ _ _ _ pi1 pi2_2 _ _) ; simpl; lia.
+      * list_simpl ; apply tens_r...
+        revert pi2_1 IHsize ; simpl ; rewrite (app_comm_cons _ _ A0) ; intros pi2_1 IHsize.
+        refine (IHsize _ _ _ _ pi1 pi2_1 _ _) ; simpl; lia.
+  - (* parr_r *)
+    destruct l1 ; inversion Heql ; subst ; list_simpl.
+    + (* main case *)
+      remember (dual (parr A0 B) :: l0) as l' ; destruct pi1; try inversion Heql'.
+      * (* ex_r *)
+        remember (parr_r _ _ _ pi2) as pi2'; clear pi2 Heqpi2' IHcut; rename pi2' into pi2.
+        simpl in IHsize.
+        destruct f; [destruct l; inversion H0 | ].
+        destruct (andb_prop _ _ e) as [Hal _]; rewrite e0 in Hal; simpl in Hal; apply andb_prop in Hal as [Hlt Hal]; apply Nat.ltb_lt in Hlt.
+        destruct (nth_split_Type n l A0) as [[la lb] Heq Hlen]...
+        replace (nth n l A0) with (tens (dual B) (dual A0)) in Heq by (destruct l; [ | app_nat_fun_unfold f l n f0; rewrite nth_indep with _ _ _ _ f0; try assumption]; now inversion H0).
+        revert pi1 pi2 IHsize; rewrite Heq; replace (parr A0 B) with (dual (tens (dual B) (dual A0))) by (simpl; now rewrite 2 bidual) ; intros pi1 pi2 IHsize.
+        enough (Perm_R (la ++ l2 ++ lb) (l0  ++ l2)) as [p [Hperm [Hlen' Heq']]].
+        { rewrite Heq'; apply ex_r...
+          apply IHsize with  (tens (dual B) (dual A0)) pi2 pi1; [ lia | ].
+          simpl in *; rewrite 2 fsize_dual; lia. }
+        transitivity (l2 ++ l0); [ | apply Perm_R_app_comm ].
+        transitivity (l2 ++ lb ++ la); [ rewrite (app_assoc _ _ la); apply Perm_R_app_comm | ]. 
+        apply Perm_R_app_head.
+        transitivity (la ++ lb) ; [ apply Perm_R_app_comm | ].
+        change l0 with (nil ++ l0); apply Perm_R_app_inv with (tens (dual B) (dual A0)).
+        split with (n :: f);rewrite<- Heq; repeat split ; [ | | symmetry]...
+      * (* tens_r *)
+        clear IHsize ; subst.
+        rewrite <- (app_nil_l (dual B :: _)) in pi1_1 ; simpl in Hc ; list_simpl.
+        refine (IHcut _ _ _ _ _ pi1_1 _); try lia.
+        rewrite <- (app_nil_l _) ; refine (IHcut _ _ _ _ _ pi1_2 _); try lia...
+    + (* commutative case *)
+      apply parr_r.
+      revert pi2 IHsize ; simpl ; rewrite (app_comm_cons l1 _ B) ; rewrite (app_comm_cons _ _ A0) ;
+        intros pi2 IHsize.
+      refine (IHsize _ _ _ _ pi1 pi2 _ _) ; simpl; lia.
+Qed.
+
+Lemma cut_elim : forall l,
+    mll_cut l ->
+    mll l.
+Proof with try assumption.
+  intros l pi.
+  induction pi; try constructor...
+  apply cut_admissible with A...
+Qed.
